src/lib/communication/DY.Lib.Communication.API.Properties.fst
@@ -8,7 +8,7 @@ open DY.Lib.Event.Typed
 open DY.Lib.State.PKI
 
 open DY.Lib.Communication.API
-open DY.Lib.Communication.API.Predicates
+open DY.Lib.Communication.API.Invariants
 
 #set-options "--fuel 0 --ifuel 0 --z3rlimit 10 --z3cliopt 'smt.qi.eager_threshold=100'"
 
@@ -21,11 +21,10 @@ open DY.Lib.Communication.API.Predicates
 val confidential_message_send:
   {|crypto_invariants|} ->
   tr:trace ->
-  sender:principal -> receiver:principal ->
   payload:bytes -> prop
-let confidential_message_send tr sender receiver payload =
+let confidential_message_send tr payload =
   exists i pk nonce.
-    let msg = encrypt_message sender receiver payload pk nonce in
+    let msg = encrypt_message payload pk nonce in
     event_at tr i (MsgSent msg) /\
     bytes_invariant tr msg
 
@@ -33,16 +32,16 @@ val confidential_message_sender_authentication:
   {|invs:protocol_invariants|} ->
   tr:trace ->
   higher_layer_preds:comm_higher_layer_event_preds ->
-  sender:principal -> receiver:principal ->
+  receiver:principal ->
   payload:bytes ->
   Lemma
   (requires
     trace_invariant tr  /\
     has_communication_layer_event_predicates invs higher_layer_preds /\
-    event_triggered tr receiver (CommConfReceiveMsg sender receiver payload)
+    event_triggered tr receiver (CommConfReceiveMsg receiver payload)
   )
   (ensures
-    event_triggered tr sender (CommConfSendMsg sender receiver payload) \/
+    (exists sender. event_triggered tr sender (CommConfSendMsg sender receiver payload)) \/
     is_publishable tr payload
   )
-let confidential_message_sender_authentication #invs tr hlp sender receiver payload = ()
+let confidential_message_sender_authentication #invs tr hlp receiver payload = ()
